code/ecdsa/Hacl.P256.fst
@@ -84,7 +84,7 @@ let ecp256dh_i_ml result scalar = Hacl.Impl.EC.DH.ecp256dh_i P256 MontLadder res
 let ecp256dh_i_radix result scalar = Hacl.Impl.EC.DH.ecp256dh_i P256 Radix result scalar
 
 
-let ecp384dh_i result scalar = Hacl.Impl.EC.DH.ecp256dh_i P384 MontLadder result scalar
+let ecp384dh_i result scalar = Hacl.Impl.EC.DH.ecp256dh_i P384 Radix result scalar
 
 
 let ecp256dh_r_public_ml result pubKey scalar = Hacl.Impl.EC.DH.ecp256dh_r_public #P256 #MontLadder result pubKey scalar
